4.4/Cyclone_LN_Extra_Lemmas_And_Automation.v
@@ -1,0 +1,192 @@
+(* 
+ This is the definition of formal syntax for Dan Grossman's Thesis, 
+  "SAFE PROGRAMMING AT THE C LEVEL OF ABSTRACTION". 
+
+  Defining type safety, page 67.
+
+*)
+
+Set Implicit Arguments.
+Set Implicit Arguments.
+Require Export Cyclone_Formal_Syntax Cyclone_Static_Semantics_Kinding_And_Context_Well_Formedness.
+Require Export Cyclone_Static_Semantics_Typing_Heap_Objects.
+Require Export Cyclone_LN_Tactics.
+Close Scope list_scope.
+Import LibEnvNotations.
+Import LVPE.LibVarPathEnvNotations.
+
+Hint Extern 1 (ok ddot) => unfold ddot.
+Hint Extern 1 (ok gdot) => unfold gdot.
+Hint Extern 1 (LVPE.okp udot) => unfold udot.
+Hint Extern 1 (ok hdot) => unfold hdot.
+
+Lemma WFD_ok:
+  forall d,  WFD d <-> ok d.
+Proof.
+  intros.
+  split.
+  introv WFDd.
+  lets: ok_push.
+  lets: get_none_inv.
+  induction* WFDd.
+  introv OKd.
+  induction* OKd.
+  constructor*.
+  apply* get_none.
+Qed.
+
+Lemma WFU_okp:
+  forall u,  WFU u -> LVPE.okp u.
+Proof.
+  introv WFUu.
+  lets: LVPE.okp_push.
+  lets: LVPE.get_none_inv.
+  induction* WFUu.
+Qed.
+
+(* not needed
+Lemma binds_ok_free:
+  forall A alpha v (d d' : env A),
+    binds alpha v d ->
+    ok d  ->
+    ok d' ->
+    ok (d & d') ->
+    alpha # d'.
+Admitted.
+
+Lemma binds_ok_binds:
+  forall A alpha v (d d' : env A),
+    binds alpha v d ->
+    ok d  ->
+    ok d' ->
+    ok (d & d') ->
+    binds alpha v (d & d').
+Proof.
+  unfold binds in *.
+  intros.
+  rewrite get_concat.
+  assert(get alpha d' = None).
+  induction d'.
+  rewrite <- empty_def.
+  apply get_empty.
+  inversion H2.
+  rewrite empty_def in H4.
+  admit. (* Should be able to invert. *)
+  admit.
+  rewrite H3.
+  assumption.
+Qed.
+
+Hint Extern 3 (binds _ _ (_ & _)) => try apply binds_ok_binds.
+*)
+
+Lemma extends_get:
+  forall A alpha (d : env A) v,
+    get alpha d = Some v ->
+    forall d', 
+      extends d d' ->
+      get alpha d' = Some v.
+Proof.
+  intros.
+  unfold extends in H0.
+  specialize (H0 alpha v).
+  induction H0.
+  reflexivity.
+  unfold binds.
+  assumption.
+Qed.
+
+Lemma extends_empty:
+  forall A (E : env A),
+    extends E empty ->
+    E = empty.
+Proof.
+  intros.
+  induction E.
+  rewrite* empty_def.
+  unfold extends in H.
+  destruct a.
+  specialize (H v a).
+  unfold binds in H.
+  rewrite get_def in H.
+  rewrite empty_def in H.
+  compute in H.
+  case_var.
+  assert (Some a = Some a); auto.
+  apply H in H0.
+  inversion H0.
+Qed.
+  
+Lemma empty_extends:
+  forall A (E : env A),
+    extends empty E.
+Proof.
+  intros.
+  induction E.
+  rewrite* empty_def.
+  unfold extends.
+  intros.
+  inversion H.
+  rewrite get_empty in H1.
+  inversion H1.
+Qed.
+
+Hint Extern 1 (extends ddot _) => unfold ddot; apply empty_extends.
+Hint Extern 1 (extends gdot _) => unfold gdot; apply empty_extends.
+Hint Extern 1 (LVPE.extends udot _) => unfold udot; apply empty_extends.
+Hint Extern 1 (extends hdot _) => unfold hdot; apply empty_extends.
+
+Lemma extends_push_both:
+  forall A (E1 E2 : env A),
+    extends E1 E2 ->
+    forall x, 
+    x # E2 ->
+     forall v, 
+       extends (E1 & x ~ v) (E2 & x ~ v).
+Proof.
+  introv E.
+  intros.
+  unfold extends.
+  intros.
+  unfold binds in H0.
+  rewrite get_push in H0.
+  case_var*.
+  inversion H0.
+  subst.
+  unfold binds.
+  rewrite get_push.
+  case_var*.
+Qed.
+
+Lemma extends_binds:
+  forall A (E E' : env A),
+    extends E E' ->
+    forall x v,
+      binds x v E ->
+      binds x v E'.
+Proof.
+  intros.
+  induction E'; auto.
+Qed.
+
+Lemma lvpe_extends_binds:
+  forall A (E E' : LVPE.varpathenv A),
+    LVPE.extends E E' ->
+    forall x v,
+      LVPE.binds x v E ->
+      LVPE.binds x v E'.
+Proof.
+  intros.
+  induction E'; auto.
+Qed.
+
+Ltac solve_binds_extends :=
+  match goal with
+    | H: extends ?u ?u', I: binds ?x ?v ?u |- binds ?x ?v ?u' =>
+      try apply extends_binds with (E:= u); auto
+    | H: LVPE.extends ?u ?u',  I: LVPE.binds ?x ?v ?u |- LVPE.binds ?x ?v ?u' =>
+      try apply lvpe_extends_binds with (E:= u); auto
+  end.
+
+Hint Extern 1 (binds _ _ _) => try solve_binds_extends.
+Hint Extern 1 (LVPE.binds _ _ _) => try solve_binds_extends.
