4.4/TermWeakeningProof.v
@@ -1,0 +1,479 @@
+(* 
+ This is the definition of formal syntax for Dan Grossman's Thesis, 
+  "SAFE PROGRAMMING AT THE C LEVEL OF ABSTRACTION". 
+
+  Defining type safety, page 67.
+
+*)
+
+Set Implicit Arguments.
+Set Implicit Arguments.
+Require Export Cyclone_Formal_Syntax Cyclone_Static_Semantics_Kinding_And_Context_Well_Formedness.
+Require Export Cyclone_Static_Semantics_Typing_Heap_Objects.
+Require Export Cyclone_Classes Cyclone_Inductions.
+Require Export Cyclone_LN_Tactics Cyclone_LN_Extra_Lemmas_And_Automation.
+Close Scope list_scope.
+Import LibEnvNotations.
+Import LVPE.LibVarPathEnvNotations.
+
+Lemma A_2_Term_Weakening_1 :
+  forall (d: Delta) (u u' : Upsilon) (g g' : Gamma)
+         (x : var) (p p' : Path) (tau tau' : Tau),
+    LVPE.extends u u' ->
+    extends g g' ->
+    WFC d u g -> 
+    WFC d u' g' ->
+    gettype u  x p tau p' tau' ->
+    gettype u' x p tau p' tau'.
+Proof.
+  intros.
+  induction H3; auto.
+  apply gettype_etype with (tau'':= tau''); auto.
+Qed.
+
+Function A_2_Term_Weakening_prop (In : Type) (H : TypJudgement In) 
+         (d : Delta) (u : Upsilon) (g : Gamma) (s : In) (t : Tau)
+         (st : typ' d u g s t) := 
+    typ' d u g s t ->
+    WFC d u g -> 
+      forall (u' : Upsilon) (g' : Gamma),
+        WFC d u' g' ->
+        LVPE.extends u u' ->
+        extends g g' ->
+        typ' d u' g' s t.
+Hint Unfold A_2_Term_Weakening_prop.
+
+
+Ltac solve_typ := 
+ match goal with 
+ | |- (styp _ _ _ (letx _ _) _)          
+	=> idtac "1"; apply_fresh_from styp_let_3_6 with fv_of_static_goal
+ | |- (styp _ _ _ (openx _ _) _)         
+	=> idtac "2"; apply_fresh_from styp_open_3_7 with fv_of_static_goal
+ | |- (styp _ _ _ (openstar _ _) _)      
+	=> idtac "3"; apply_fresh_from styp_openstar_3_8 with fv_of_static_goal
+ | |- (rtyp _ _ _ (pack _ _ _) _)       
+	=> idtac "4"; apply_fresh_from SR_3_12 with fv_of_static_goal
+ | |- (rtyp _ _ _ (f_e (ufun _ _)) _)    
+	=> idtac "5"; apply_fresh_from SR_3_14 with fv_of_static_goal
+ | |- (rtyp _ _ _ (f_e (dfun _ _ _ )) _) 
+	=> idtac "6"; apply_fresh_from SR_3_13 with fv_of_static_goal
+ | |- (ltyp _ _ _ (p_e _ _) _) =>
+   idtac "12"; applys SL_3_1
+ | |- (rtyp ?a ?b ?c (p_e ?d ?e) ?f) =>
+   idtac "13 a b c d e f"; applys SR_3_1
+ | |- (ltyp _ _ _  (dot (p_e _ _) zero_pe) _) =>
+   idtac "14"; applys SL_3_3
+ | |- (ltyp _ _ _ (dot (p_e _ _) one_pe)  _)  =>
+   idtac "15"; applys SL_3_4
+ | |- (rtyp _ _ _ (dot _ zero_pe) _)          =>
+   idtac "16"; applys SR_3_3
+ | |- (rtyp _ _ _ (dot _ one_pe)  _)          =>
+   idtac "17"; applys SR_3_4
+ | |- (styp _ _ _ (e_s _) _)                  =>
+   idtac "18"; applys styp_e_3_1
+ | |- (rtyp _ _ _ (appl _ _) _)               =>
+   idtac "19"; applys SR_3_9
+end.
+
+Lemma gettype_weakening:
+  forall u u' x tau' p tau,
+  gettype u x nil tau' p tau ->
+  LVPE.extends u u' ->
+  gettype u' x nil tau' p tau.
+Admitted.
+
+
+Lemma A_2_Term_Weakening_2:
+  forall (d : Delta) (u : Upsilon) (g : Gamma) (s : E) (t : Tau) (ty : typ' d u g s t),
+   A_2_Term_Weakening_prop LtypJudgement d u g s t ty.
+Proof.
+  intros.
+  Typ_Induction ltyp_ind_mutual A_2_Term_Weakening_prop; intros; auto.
+  admit.
+  admit.
+  admit.
+  apply SL_3_1 with (tau':=tau'); auto.
+  apply gettype_weakening with (u:= u0); auto.
+  apply SL_3_3 with (t1:= t1); auto.
+  apply SL_3_4 with (t0:= t0); auto.
+  apply SR_3_1 with (tau':= tau'); auto.
+  apply gettype_weakening with (u:= u0); auto.
+  apply SR_3_3 with (t1:= t1); auto.
+  apply SR_3_4 with (t0:= t0); auto.
+  apply SR_3_9 with (tau':= tau'); auto.
+  apply SR_3_11 with (k:=k) (tau':= tau'); auto.
+  admit.
+  apply SR_3_13 with (L:=        ((((((((((((((L \u T.fv t) \u T.fv tau) \u T.fv tau') \u TM.fv_st s0) \u TM.fv_e s) \u
+                TTM.fv_st s0) \u TTM.fv_e s) \u fv_delta d) \u 
+             fv_delta d0) \u fv_gamma g) \u fv_gamma g0) \u fv_gamma g') \u 
+         fv_upsilon u) \u fv_upsilon u0) \u fv_upsilon u'). auto.
+  
+  
+  apply styp_let_3_6 with (tau':= tau') (L:= 
+((((((((((((((((L \u T.fv t) \u T.fv tau) \u T.fv tau') \u TM.fv_st s0) \u
+                   TM.fv_e s) \u TM.fv_e e) \u TTM.fv_st s0) \u 
+                TTM.fv_e s) \u TTM.fv_e e) \u fv_delta d) \u fv_delta d0) \u 
+            fv_gamma g) \u fv_gamma g0) \u fv_gamma g') \u fv_upsilon u) \u 
+        fv_upsilon u0) \u fv_upsilon u').
+  intros.
+  auto.
+  apply_fresh_from styp_let_3_6 with fv_of_static_goal.
+  solve_typ.
+
+  admit.
+  admit.
+  admit.
+
+  admit.
+  apply SL_3_3 with (t1:= t1); auto.
+  apply SL_3_4 with (t0:= t0); auto.
+
+  
+
+barrier .
+
+
+
+Lemma A_2_Term_Weakening_3:
+  forall (d: Delta) (u : Upsilon) (g : Gamma)  (e : E) (tau : Tau),
+    rtyp d u g e tau ->
+    WFC d u g -> 
+      forall (u' : Upsilon) (g' : Gamma),
+        WFC d u' g' ->
+        U.extends u u' = true ->
+        G.extends g g' = true ->
+        WFC d u g' ->
+        rtyp d u' g' e tau.
+Proof.
+(*
+  intros d u g e tau ltypder.
+  apply (rtyp_ind_mutual
+           (fun (d : Delta) (u : Upsilon) (g : Gamma) (t : Tau) (s : St)
+                (st : styp d u g t s) => 
+              WFC d u g -> 
+              forall (u' : Upsilon) (g' : Gamma),
+                WFC d u' g' ->
+                WFC d (u ++ u') (g ++ g') ->
+                styp d (u ++ u') (g ++ g') t s)
+           (fun (d : Delta) (u : Upsilon) (g : Gamma) (e : E) (t : Tau) 
+                (lt : ltyp d u g  e t) =>
+              WFC d u g -> 
+              forall (u' : Upsilon) (g' : Gamma),
+                WFC d u' g' ->
+                WFC d (u ++ u') (g ++ g') ->
+                ltyp d (u ++ u') (g ++ g') e t)
+           (fun (d : Delta) (u : Upsilon) (g : Gamma) (e : E) (t : Tau) 
+                (rt : rtyp d u g e t) =>
+              WFC d u g -> 
+              forall (u' : Upsilon) (g' : Gamma),
+                WFC d u' g' ->
+                WFC d (u ++ u') (g ++ g') ->
+                rtyp d (u ++ u') (g ++ g') e t)).
+(*
+  Case "styp_e_3_1".
+   intros.
+   constructor.
+   apply H with (u':= u') (g':= g') in H1; try assumption.
+  Case "styp_return_3_2".
+   intros.
+   constructor.
+   apply H with (u':= u') (g':= g') in H1; try assumption.
+  Case "styp_seq_3_3".
+   intros.
+   constructor.
+   apply H with (u':= u') (g':= g') in H1; try assumption.
+   apply H0 with (u':= u') (g':= g') in H1; try assumption.
+  Case "styp_while_3_4".
+   intros.
+   constructor.
+   apply H with (u':= u') (g':= g') in H1; try assumption.
+   apply H0 with (u':= u') (g':= g') in H1; try assumption.
+  Case "styp_if_3_5".
+   intros.
+   constructor.
+   apply H with (u':= u') (g':= g') in H2; try assumption.
+   apply H0 with (u':= u') (g':= g') in H2; try assumption.
+   apply H1 with (u':= u') (g':= g') in H2; try assumption.
+  Case "styp_let_3_6".
+   intros.
+   apply styp_let_3_6 with (tau':=tau'); try assumption.
+   AdmitAlphaConversion.
+   inversion H2; try assumption.
+   assert (Z: WFC d0 u0 ([(x, tau')] ++ g0)). (* How do I get this ? *)
+   constructor; try assumption.
+   constructor; try assumption.
+   admit.
+   admit.
+   admit.
+   admit.
+   admit.
+   (* 
+   apply H with (u':= u') (g':= g') in Z; try assumption.
+   admit.
+   apply H0 with (u':= u') (g':= g') in H1; try assumption.
+   *)
+  Case "styp_open_3_7".
+   admit. (* Will have the similar problems with let. *)
+  Case "styp_openstar_3_8".
+   admit. (* Will have the similar problems with let. *)
+  Case "SL_3_1".
+  (* Should use the previous theorem.
+   intros.
+   apply SL_3_1 with (tau':= tau0); try assumption.
+   apply getG_Some_Weakening; try assumption.
+   apply gettype_weakening; try assumption.
+   inversion H; try assumption.
+   inversion H1; try assumption.
+   *)
+  admit.
+  Case "SL_3_2".
+   intros.
+   admit. (* constructor; try assumption. *)
+   (* apply H with (u':= u') (g':= g') in H0; try assumption. *)
+  Case "SL_3_3".
+   intros.
+   apply SL_3_3 with (t1:= t1); try assumption.
+   apply H with (u':= u') (g':= g') in H0; try assumption.
+  Case "SL_3_4".
+   intros.
+   apply SL_3_4 with (t0:= t0); try assumption.
+   apply H with (u':= u') (g':= g') in H0; try assumption.
+  Case "SR_3_1".
+   intros.
+   apply SR_3_1 with (tau':= tau'); try assumption.
+   apply getG_Some_Weakening; try assumption.
+   apply gettype_weakening; try assumption.
+   inversion H; try assumption.
+   inversion H1; try assumption.
+  Case "SR_3_2".
+   intros.
+   constructor; try assumption.
+   apply H with (u':= u') (g':= g') in H0; try assumption.
+  Case "SR_3_3".
+   intros.
+   apply SR_3_3 with (t1:= t1); try assumption.
+   apply H with (u':= u') (g':= g') in H0; try assumption.
+  Case "SR_3_4".
+   intros.
+   apply SR_3_4 with (t0:= t0); try assumption.
+   apply H with (u':= u') (g':= g') in H0; try assumption.
+  Case "SR_3_5".
+   intros.
+   constructor; try assumption.
+  Case "SR_3_6".
+   intros.
+   constructor; try assumption.
+   apply H with (u':= u') (g':= g') in H0; try assumption.
+  Case "SR_3_7".
+   intros.
+   constructor; try assumption.
+   apply H with (u':= u') (g':= g') in H1; try assumption.
+   apply H0 with (u':= u') (g':= g') in H1; try assumption.
+  Case "SR_3_8".
+   intros.
+   constructor; try assumption.
+   apply H with (u':= u') (g':= g') in H1; try assumption.
+   apply H0 with (u':= u') (g':= g') in H1; try assumption.
+  Case "SR_3_9".
+   intros.
+   apply SR_3_9 with (tau':= tau'); try assumption.
+   apply H with (u':= u') (g':= g') in H1; try assumption.
+   apply H0 with (u':= u') (g':= g') in H1; try assumption.
+  Case "SR_3_10".
+   intros.
+   constructor; try assumption.
+   apply H with (u':= u') (g':= g') in H1; try assumption.
+  Case "SR_3_11".
+   intros.
+   apply SR_3_11 with (k:=k); try assumption.
+   apply H with (u':= u') (g':= g') in H1; try assumption.
+  Case "SR_3_12".
+   intros.
+   constructor; try assumption.
+   apply H with (u':= u') (g':= g') in H1; try assumption.
+  Case "SR_3_13".
+   intros.
+   constructor; try assumption.
+   apply H with (u':= u') (g':= g') in H1; try assumption.
+   AdmitAlphaConversion.
+   admit.
+   admit.
+   apply H with (u':= u') (g':= g') in H1; try assumption.
+   admit.
+   admit.
+  Case "SR_3_14".
+   admit.
+  Case "base".
+   assumption.
+Qed.
+*)
+*)
+Admitted.
+
+Lemma A_2_Term_Weakening_4:
+  forall (d: Delta) (u : Upsilon) (g : Gamma)  (s : St) (tau : Tau),
+    styp d u g tau s ->
+    WFC d u g -> 
+      forall (u' : Upsilon) (g' : Gamma),
+        WFC d u' g' ->
+        U.extends u u' = true ->
+        G.extends g g' = true ->
+        WFC d u' g' ->
+        styp d u' g' tau s.
+Proof.
+(*
+  intros d u g e tau ltypder.
+  apply (styp_ind_mutual
+           (fun (d : Delta) (u : Upsilon) (g : Gamma) (t : Tau) (s : St)
+                (st : styp d u g t s) => 
+              WFC d u g -> 
+              forall (u' : Upsilon) (g' : Gamma),
+                WFC d u' g' ->
+                WFC d (u ++ u') (g ++ g') ->
+                styp d (u ++ u') (g ++ g') t s)
+           (fun (d : Delta) (u : Upsilon) (g : Gamma) (e : E) (t : Tau) 
+                (lt : ltyp d u g  e t) =>
+              WFC d u g -> 
+              forall (u' : Upsilon) (g' : Gamma),
+                WFC d u' g' ->
+                WFC d (u ++ u') (g ++ g') ->
+                ltyp d (u ++ u') (g ++ g') e t)
+           (fun (d : Delta) (u : Upsilon) (g : Gamma) (e : E) (t : Tau) 
+                (rt : rtyp d u g e t) =>
+              WFC d u g -> 
+              forall (u' : Upsilon) (g' : Gamma),
+                WFC d u' g' ->
+                WFC d (u ++ u') (g ++ g') ->
+                rtyp d (u ++ u') (g ++ g') e t)).
+  Case "styp_e_3_1".
+   intros.
+   apply styp_e_3_1 with (tau':= tau').
+   apply H with (u':= u') (g':= g') in H1; try assumption.
+  Case "styp_return_3_2".
+   intros.
+   constructor.
+   apply H with (u':= u') (g':= g') in H1; try assumption.
+  Case "styp_seq_3_3".
+   intros.
+   constructor.
+   apply H with (u':= u') (g':= g') in H1; try assumption.
+   apply H0 with (u':= u') (g':= g') in H1; try assumption.
+  Case "styp_while_3_4".
+   intros.
+   constructor.
+   apply H with (u':= u') (g':= g') in H1; try assumption.
+   apply H0 with (u':= u') (g':= g') in H1; try assumption.
+  Case "styp_if_3_5".
+   intros.
+   constructor.
+   apply H with (u':= u') (g':= g') in H2; try assumption.
+   apply H0 with (u':= u') (g':= g') in H2; try assumption.
+   apply H1 with (u':= u') (g':= g') in H2; try assumption.
+  Case "styp_let_3_6".
+   admit.
+   (* 
+   intros.
+   apply styp_let_3_6 with (tau':=tau'); try assumption.
+   AdmitAlphaConversion.
+   inversion H2; try assumption.
+   assert (Z: WFC d0 u0 ([(x, tau')] ++ g0)). (* How do I get this ? *)
+   constructor; try assumption.
+   constructor; try assumption.
+
+   apply H with (u':= u') (g':= g') in Z; try assumption.
+   admit.
+   apply H0 with (u':= u') (g':= g') in H1; try assumption.
+    *)
+  Case "styp_open_3_7".
+   admit. (* Will have the similar problems with let. *)
+  Case "styp_openstar_3_8".
+   admit. (* Will have the similar problems with let. *)
+  Case "SL_3_1".
+   intros.
+   apply SL_3_1 with (tau':=tau'); try assumption.
+   apply getG_Some_Weakening; try assumption.
+   apply gettype_weakening; try assumption.
+   inversion H; try assumption.
+   inversion H1; try assumption.
+  Case "SL_3_2".
+   intros.
+   constructor; try assumption.
+   apply H with (u':= u') (g':= g') in H0; try assumption.
+  Case "SL_3_3".
+   intros.
+   apply SL_3_3 with (t1:= t1); try assumption.
+   apply H with (u':= u') (g':= g') in H0; try assumption.
+  Case "SL_3_4".
+   intros.
+   apply SL_3_4 with (t0:= t0); try assumption.
+   apply H with (u':= u') (g':= g') in H0; try assumption.
+  Case "SR_3_1".
+   intros.
+   apply SR_3_1 with (tau':= tau'); try assumption.
+   apply getG_Some_Weakening; try assumption.
+   apply gettype_weakening; try assumption.
+   inversion H; try assumption.
+   inversion H1; try assumption.
+  Case "SR_3_2".
+   intros.
+   constructor; try assumption.
+   apply H with (u':= u') (g':= g') in H0; try assumption.
+  Case "SR_3_3".
+   intros.
+   apply SR_3_3 with (t1:= t1); try assumption.
+   apply H with (u':= u') (g':= g') in H0; try assumption.
+  Case "SR_3_4".
+   intros.
+   apply SR_3_4 with (t0:= t0); try assumption.
+   apply H with (u':= u') (g':= g') in H0; try assumption.
+  Case "SR_3_5".
+   intros.
+   constructor; try assumption.
+  Case "SR_3_6".
+   intros.
+   constructor; try assumption.
+   apply H with (u':= u') (g':= g') in H0; try assumption.
+  Case "SR_3_7".
+   intros.
+   constructor; try assumption.
+   apply H with (u':= u') (g':= g') in H1; try assumption.
+   apply H0 with (u':= u') (g':= g') in H1; try assumption.
+  Case "SR_3_8".
+   intros.
+   constructor; try assumption.
+   apply H with (u':= u') (g':= g') in H1; try assumption.
+   apply H0 with (u':= u') (g':= g') in H1; try assumption.
+  Case "SR_3_9".
+   intros.
+   apply SR_3_9 with (tau':= tau'); try assumption.
+   apply H with (u':= u') (g':= g') in H1; try assumption.
+   apply H0 with (u':= u') (g':= g') in H1; try assumption.
+  Case "SR_3_10".
+   intros.
+   constructor; try assumption.
+   apply H with (u':= u') (g':= g') in H1; try assumption.
+  Case "SR_3_11".
+   intros.
+   apply SR_3_11 with (k:=k); try assumption.
+   apply H with (u':= u') (g':= g') in H1; try assumption.
+  Case "SR_3_12".
+   intros.
+   constructor; try assumption.
+   apply H with (u':= u') (g':= g') in H1; try assumption.
+  Case "SR_3_13".
+   intros.
+   constructor; try assumption.
+   apply H with (u':= u') (g':= g') in H1; try assumption.
+   AdmitAlphaConversion.
+   admit.
+   admit.
+   apply H with (u':= u') (g':= g') in H1; try assumption.
+   admit.
+   admit.
+  Case "SR_3_14".
+   admit.
+  Case "base".
+   assumption.
+*)
+Admitted.
