4.4/genenv/LibEValue.v
@@ -1,0 +1,22 @@
+Set Implicit Arguments.
+Require Import Cyclone_Formal_Syntax.
+Require Import LibValueType.
+Require Import TLC.LibReflect TLC.LibFset.
+
+Module EValue : ValueType.
+
+Definition value := E.
+
+Lemma value_inhab : Inhab E.
+Proof using. apply (prove_Inhab (i_e (i_i 0))). Qed.
+
+Lemma value_comp : Comparable E.
+Admitted.
+
+Instance value_comparable : Comparable value := value_comp.
+
+Definition values := fset E.
+(* How do I get var without too much ? 
+Function fv (v : value) := VariablesType.vars.
+*)
+End EValue.
