4.4/genenv/LibFresh.v
@@ -1,0 +1,152 @@
+Require Import TLC.LibTactics TLC.LibOption TLC.LibList TLC.LibProd TLC.LibLogic TLC.LibReflect TLC.LibFset.
+Require Import LibNotIn.
+
+Fixpoint fresh (A: Type) (L : fset A) (n : nat) (xs : list A) {struct xs} : Prop :=
+  match xs, n with
+  | nil, O => True
+  | x::xs', S n' => x \notin L /\ fresh A (L \u \{x}) n' xs'
+  | _,_ => False
+  end.
+
+Hint Extern 1 (fresh _ _ _) => simpl.
+
+Lemma fresh_union_r : forall (A : Type) xs L1 L2 n,
+  fresh A (L1 \u L2) n xs -> fresh A L1 n xs /\ fresh A L2 n xs.
+Proof using.
+  induction xs; simpl; intros; destruct n;
+  tryfalse*. auto.
+  destruct H. split; split; auto.
+  forwards*: (@IHxs (L1 \u \{a}) L2 n).
+   rewrite union_comm.
+   rewrite union_comm_assoc.
+   rewrite* union_assoc.
+  forwards*: (@IHxs L1 (L2 \u \{a}) n).
+   rewrite* union_assoc.
+Qed.
+
+Lemma fresh_union_r1 : forall A xs L1 L2 n,
+  fresh A (L1 \u L2) n xs -> fresh A L1 n xs.
+Proof using. intros. forwards*: fresh_union_r. Qed.
+
+Lemma fresh_union_r2 : forall A xs L1 L2 n,
+  fresh A (L1 \u L2) n xs -> fresh A L2 n xs.
+Proof using. intros. forwards*: fresh_union_r. Qed.
+
+Lemma fresh_union_l : forall A xs L1 L2 n,
+  fresh A L1 n xs -> fresh A L2 n xs -> fresh A (L1 \u L2) n xs.
+Proof using.
+  induction xs; simpl; intros; destruct n; tryfalse*. auto.
+  destruct H. destruct H0. split~.
+  forwards~ K: (@IHxs (L1 \u \{a}) (L2 \u \{a}) n).
+  rewrite <- (union_same \{a}).
+  rewrite union_assoc.
+  rewrite <- (union_assoc L1).
+  rewrite (union_comm L2).
+  rewrite (union_assoc L1).
+  rewrite* <- union_assoc.
+Qed.
+
+Lemma fresh_empty : forall A L n xs,
+  fresh A L n xs -> fresh A \{} n xs.
+Proof using.
+  intros. rewrite <- (union_empty_r L) in H.
+  destruct* (fresh_union_r _ _ _ _ _ H).
+Qed.
+
+Lemma fresh_length : forall A L n xs,
+  fresh A L n xs -> n = length xs.
+Proof using.
+  intros. gen n L. induction xs; simpl; intros n L Fr;
+    destruct n; tryfalse*.
+  auto.
+  rew_length. rewrite* <- (@IHxs n (L \u \{a})).
+Qed.
+
+Lemma fresh_resize : forall A L n xs,
+  fresh A L n xs -> forall m, m = n -> fresh A L m xs.
+Proof using.
+  introv Fr Eq. subst~.
+Qed.
+
+Lemma fresh_resize_length : forall A L n xs,
+  fresh A L n xs -> fresh A L (length xs) xs.
+Proof using.
+  introv Fr. rewrite* <- (fresh_length _ _ _ _ Fr).
+Qed.
+
+Implicit Arguments fresh_union_r [xs L1 L2 n].
+Implicit Arguments fresh_union_r1 [xs L1 L2 n].
+Implicit Arguments fresh_union_r2 [xs L1 L2 n].
+Implicit Arguments fresh_union_l [xs L1 L2 n].
+Implicit Arguments fresh_empty  [L n xs].
+Implicit Arguments fresh_length [L n xs].
+Implicit Arguments fresh_resize [L n xs].
+Implicit Arguments fresh_resize_length [L n xs].
+
+Lemma fresh_single_notin : forall A x xs n,
+  fresh A \{x} n xs ->
+  x \notin from_list xs.
+Proof using.
+  induction xs; destruct n; introv F; simpl in F; tryfalse.
+  rewrite~ from_list_nil.
+  destruct F as [Fr F']. lets [? ?]: (fresh_union_r _ F').
+   specializes IHxs n. rewrite~ from_list_cons.
+Qed.
+
+Ltac fresh_solve_target_from E n xs H :=
+  match type of H with
+  | fresh E n xs => constr:(H)
+  | fresh E ?m xs =>
+      match n with
+      | length xs => constr:(fresh_resize_length H)
+      | _ =>
+         match goal with
+         | Eq: m = n |- _ => constr:(fresh_resize H _ (sym_eq Eq))
+         | Eq: n = m |- _ => constr:(fresh_resize H _ Eq)
+         end
+      end
+  | fresh (?F \u ?G) ?m xs =>
+     let H' :=
+        match F with
+        | context [E] => constr:(fresh_union_r1 H)
+        | _ => match G with
+          | context [E] => constr:(fresh_union_r2 H)
+          | _ => fail 20
+          end
+        end in
+     fresh_solve_target_from E n xs H'
+  end.
+
+Ltac fresh_solve_target E n xs :=
+  match goal with H: fresh ?L _ xs |- _ =>
+    match L with context[E] =>
+      let F := fresh_solve_target_from E n xs H in
+      apply F
+    end
+  end.
+
+Ltac fresh_solve_one :=
+  match goal with
+  | |- fresh ?E ?n ?xs =>
+    fresh_solve_target E n xs
+  | |- fresh \{} ?n ?xs =>
+    match goal with H: fresh ?F ?m xs |- _ =>
+      apply (fresh_empty H);
+      fresh_solve_target F n xs
+    end
+  end.
+
+Ltac fresh_simpl :=
+  try match goal with |- fresh (_ \u _) _ _ =>
+    apply fresh_union_l; fresh_simpl end.
+
+Ltac fresh_solve_by_notins :=
+  simpl; splits; try notin_solve.
+
+Ltac fresh_solve :=
+  fresh_simpl;
+  first [ fresh_solve_one
+        | fresh_solve_by_notins
+        | idtac ].
+
+Hint Extern 1 (fresh _ _ _) => fresh_solve.
