4.4/genenv/LibKeyType.v
@@ -1,0 +1,38 @@
+(**************************************************************************
+* TLC: A library for Coq                                                  *
+* Keys for environment signature. 
+**************************************************************************)
+
+Set Implicit Arguments.
+Require Import TLC.LibTactics TLC.LibList TLC.LibLogic TLC.LibNat TLC.LibEpsilon TLC.LibReflect.
+Require Export TLC.LibFset.
+Require Export LibFresh.
+
+(** * Abstract Definition of Key for an environment. *)
+
+Module Type KeyType.
+
+(** We leave the type of variables abstract. *)
+
+Parameter key : Set.
+
+(** This type is inhabited. *)
+
+Parameter key_inhab : Inhab key.
+
+(** This type is comparable. *)
+Parameter key_comp : Comparable key.
+Instance  key_comparable : Comparable key := key_comp.
+
+(** We can build sets of variables. *)
+
+Definition keys := fset key.
+
+(** Finally, we have a means of generating fresh variables. *)
+
+Parameter key_gen : keys -> key.
+Parameter key_gen_spec : forall E, (key_gen E) \notin E.
+Parameter key_fresh : forall (L : keys), { x : key | x \notin L }.
+
+Axiom key_freshes : forall L n, { xs : list key | fresh key L n xs}.
+End KeyType.
